More progress in reorganization. This is still a broken commit.

SeparationLogic/Semantics/DownwardsSemantics.v
@@ -7,6 +7,8 @@ Require Import Logic.SeparationLogic.Syntax.
 Require Import Logic.PropositionalLogic.KripkeModel.
 Require Import Logic.SeparationLogic.Model.SeparationAlgebra.
 Require Import Logic.SeparationLogic.Model.OrderedSA.
+Require Logic.SeparationLogic.Semantics.WeakSemantics.
+Require Logic.SeparationLogic.Semantics.StrongSemantics.
 
 Local Open Scope logic_base.
 Local Open Scope syntax.
@@ -14,74 +16,6 @@ Local Open Scope kripke_model.
 Import SeparationLogicNotation.
 Import KripkeModelFamilyNotation.
 Import KripkeModelNotation_Intuitionistic.
-
-Module Semantics.
-
-Definition sepcon {worlds: Type} {R: Relation worlds} {J: Join worlds} (X: Ensemble worlds) (Y: Ensemble worlds): Ensemble worlds :=
-  fun m => exists m0 m1 m2, m0 <= m /\ join m1 m2 m0 /\ X m1 /\ Y m2.
-
-Definition wand {worlds: Type} {J: Join worlds} (X: Ensemble worlds) (Y: Ensemble worlds): Ensemble worlds :=
-  fun m => forall m1 m2, join m m1 m2 -> X m1 -> Y m2.
-
-Definition emp {worlds: Type} {R: Relation worlds} {J: Join worlds}: Ensemble worlds := increasing.
-
-Lemma sepcon_closed
-      {worlds: Type}
-      {R: Relation worlds}
-      {kiM: KripkeIntuitionisticModel worlds}
-      {J: Join worlds}:
-  forall (X: Ensemble worlds) (Y: Ensemble worlds),
-    upwards_closed_Kdenote X ->
-    upwards_closed_Kdenote Y ->
-    upwards_closed_Kdenote (sepcon X Y).
-Proof.
-  intros.
-  hnf; intros.
-  hnf in H2 |- *.
-  destruct H2 as [n0 [n1 [n2 [? [? [? ?]]]]]].
-  exists n0, n1, n2; split; [| split; [| split]]; auto.
-  etransitivity; eauto.
-Qed.
-
-Lemma wand_closed
-      {worlds: Type}
-      {R: Relation worlds}
-      {kiM: KripkeIntuitionisticModel worlds}
-      {J: Join worlds}
-      {SA: SeparationAlgebra worlds}
-      {dSA: DownwardsClosedSeparationAlgebra worlds}:
-  forall (X: Ensemble worlds) (Y: Ensemble worlds),
-    upwards_closed_Kdenote X ->
-    upwards_closed_Kdenote Y ->
-    upwards_closed_Kdenote (wand X Y).
-Proof.
-  intros.
-  hnf; intros.
-  hnf in H2 |- *.
-  intros.
-  destruct (join_Korder_down _ _ _ _ _ H3 H1 ltac:(reflexivity)) as [m2' [? ?]].
-  apply (H0 m2'); auto.
-  apply (H2 m1); auto.
-Qed.
-
-Lemma emp_closed
-      {worlds: Type}
-      {R: Relation worlds}
-      {kiM: KripkeIntuitionisticModel worlds}
-      {J: Join worlds}
-      {SA: SeparationAlgebra worlds}
-      {dSA: DownwardsClosedSeparationAlgebra worlds}:
-  upwards_closed_Kdenote emp.
-Proof.
-  intros.
-  hnf; intros.
-  hnf in H0 |- *.
-  intros.
-  destruct (join_Korder_down _ _ _ _ _ H1 H ltac:(reflexivity)) as [n'' [? ?]].
-  etransitivity; eauto.
-Qed.
-
-End Semantics.
 
 Class SeparatingSemantics
       (L: Language)
@@ -93,8 +27,8 @@ Class SeparatingSemantics
       {J: Join (Kworlds M)}
       (SM: Semantics L MD): Type :=
 {
-  denote_sepcon: forall x y, Same_set _ (Kdenotation M (x * y)) (Semantics.sepcon (Kdenotation M x) (Kdenotation M y));
-  denote_wand: forall x y, Same_set _ (Kdenotation M (x -* y)) (Semantics.wand (Kdenotation M x) (Kdenotation M y))
+  denote_sepcon: forall x y, Same_set _ (Kdenotation M (x * y)) (StrongSemantics.sepcon (Kdenotation M x) (Kdenotation M y));
+  denote_wand: forall x y, Same_set _ (Kdenotation M (x -* y)) (WeakSemantics.wand (Kdenotation M x) (Kdenotation M y))
 }.
 
 Class EmpSemantics
@@ -107,7 +41,7 @@ Class EmpSemantics
       {R: Relation (Kworlds M)}
       {J: Join (Kworlds M)}
       (SM: Semantics L MD): Type :=
-  denote_emp: Same_set _ (Kdenotation M emp) Semantics.emp.
+  denote_emp: Same_set _ (Kdenotation M emp) WeakSemantics.emp.
 
 Lemma sat_sepcon
       {L: Language}
