SeparationLogic/Semantics/WeakSemantics.v
@@ -1,22 +1,22 @@
 Require Import Coq.Logic.Classical_Prop.
 Require Import Coq.Classes.RelationClasses.
 Require Import Coq.Relations.Relation_Definitions.
+Require Import Coq.Sets.Ensembles.
 Require Import Logic.lib.Coqlib.
-Require Import Logic.GeneralLogic.Base.
-Require Import Logic.SeparationLogic.Syntax.
 Require Import Logic.PropositionalLogic.KripkeModel.
 Require Import Logic.SeparationLogic.Model.SeparationAlgebra.
 Require Import Logic.SeparationLogic.Model.OrderedSA.
 
-Local Open Scope logic_base.
-Local Open Scope syntax.
 Local Open Scope kripke_model.
-Import SeparationLogicNotation.
-Import KripkeModelFamilyNotation.
 Import KripkeModelNotation_Intuitionistic.
 
 Definition sepcon {worlds: Type} {J: Join worlds} (X: Ensemble worlds) (Y: Ensemble worlds): Ensemble worlds :=
   fun m => exists m1 m2, join m1 m2 m /\ X m1 /\ Y m2.
+
+Definition wand {worlds: Type} {J: Join worlds} (X: Ensemble worlds) (Y: Ensemble worlds): Ensemble worlds :=
+  fun m => forall m1 m2, join m m1 m2 -> X m1 -> Y m2.
+
+Definition emp {worlds: Type} {R: Relation worlds} {J: Join worlds}: Ensemble worlds := increasing.
 
 Lemma sepcon_closed
       {worlds: Type}
@@ -39,4 +39,42 @@ Proof.
   split; [| split]; auto.
   + apply (H n1); auto.
   + apply (H0 n2); auto.
+Qed.
+
+Lemma wand_closed
+      {worlds: Type}
+      {R: Relation worlds}
+      {kiM: KripkeIntuitionisticModel worlds}
+      {J: Join worlds}
+      {SA: SeparationAlgebra worlds}
+      {dSA: DownwardsClosedSeparationAlgebra worlds}:
+  forall (X: Ensemble worlds) (Y: Ensemble worlds),
+    upwards_closed_Kdenote X ->
+    upwards_closed_Kdenote Y ->
+    upwards_closed_Kdenote (wand X Y).
+Proof.
+  intros.
+  hnf; intros.
+  hnf in H2 |- *.
+  intros.
+  destruct (join_Korder_down _ _ _ _ _ H3 H1 ltac:(reflexivity)) as [m2' [? ?]].
+  apply (H0 m2'); auto.
+  apply (H2 m1); auto.
+Qed.
+
+Lemma emp_closed
+      {worlds: Type}
+      {R: Relation worlds}
+      {kiM: KripkeIntuitionisticModel worlds}
+      {J: Join worlds}
+      {SA: SeparationAlgebra worlds}
+      {dSA: DownwardsClosedSeparationAlgebra worlds}:
+  upwards_closed_Kdenote emp.
+Proof.
+  intros.
+  hnf; intros.
+  hnf in H0 |- *.
+  intros.
+  destruct (join_Korder_down _ _ _ _ _ H1 H ltac:(reflexivity)) as [n'' [? ?]].
+  etransitivity; eauto.
 Qed.
